lib/monads/trace: copy in definitions and rules from nondet
This fills out the trace monad rule set by copying in as many
definitions and rules as possible from the nondet monad. Most of these
do not immediately work for the trace monad, see the next commit for the
required changes.

Signed-off-by: Corey Lewis <corey.lewis@proofcraft.systems>

lib/Monads/trace/Trace_Monad.thy
@@ -46,6 +46,23 @@ text \<open>
   pair of result and state when the computation did not fail.\<close>
 type_synonym ('s, 'a) tmonad = "'s \<Rightarrow> ((tmid \<times> 's) list \<times> ('s, 'a) tmres) set"
 
+text \<open>
+  Print the type @{typ "('s,'a) nondet_monad"} instead of its unwieldy expansion.
+  Needs an AST translation in code, because it needs to check that the state variable
+  @{typ 's} occurs twice. This comparison is not guaranteed to always work as expected
+  (AST instances might have different decoration), but it does seem to work here.\<close>
+print_ast_translation \<open>
+  let
+    fun monad_tr _ [t1, Ast.Appl [Ast.Constant @{type_syntax prod},
+                          Ast.Appl [Ast.Constant @{type_syntax set},
+                            Ast.Appl [Ast.Constant @{type_syntax prod}, t2, t3]],
+                          Ast.Constant @{type_syntax bool}]] =
+      if t3 = t1
+      then Ast.Appl [Ast.Constant @{type_syntax "nondet_monad"}, t1, t2]
+      else raise Match
+  in [(@{type_syntax "fun"}, monad_tr)] end
+\<close>
+
 text \<open>Returns monad results, ignoring failures and traces.\<close>
 definition mres :: "((tmid \<times> 's) list \<times> ('s, 'a) tmres) set \<Rightarrow> ('a \<times> 's) set" where
   "mres r = Result -` (snd ` r)"
@@ -124,6 +141,12 @@ text \<open>
   FIXME: The @{text select_f} function was left out here until we figure
   out what variant we actually need.\<close>
 
+text \<open>@{text select_state} takes a relationship between
+  states, and outputs nondeterministically a state
+  related to the input state.\<close>
+definition state_select :: "('s \<times> 's) set \<Rightarrow> ('s, unit) nondet_monad" where
+  "state_select r \<equiv> \<lambda>s. ((\<lambda>x. ((), x)) ` {s'. (s, s') \<in> r}, \<not> (\<exists>s'. (s, s') \<in> r))"
+
 subsection "Failure"
 
 text \<open>
@@ -184,6 +207,13 @@ text \<open>
   return @{text v} if it returns @{term "Some v"}.\<close>
 definition gets_the :: "('s \<Rightarrow> 'a option) \<Rightarrow> ('s, 'a) tmonad" where
   "gets_the f \<equiv> gets f >>= assert_opt"
+
+text \<open>
+  Get a map (such as a heap) from the current state and apply an argument to the map.
+  Fail if the map returns @{const None}, otherwise return the value.\<close>
+definition
+  gets_map :: "('s \<Rightarrow> 'a \<Rightarrow> 'b option) \<Rightarrow> 'a \<Rightarrow> ('s, 'b) nondet_monad" where
+  "gets_map f p \<equiv> gets f >>= (\<lambda>m. assert_opt (m p))"
 
 
 subsection \<open>The Monad Laws\<close>
@@ -490,6 +520,10 @@ text \<open>The same for the exception monad:\<close>
 definition liftME :: "('a \<Rightarrow> 'b) \<Rightarrow> ('s,'e+'a) tmonad \<Rightarrow> ('s,'e+'b) tmonad" where
   "liftME f m \<equiv> doE x \<leftarrow> m; returnOk (f x) odE"
 
+text \<open> Execute @{term f} for @{term "Some x"}, otherwise do nothing. \<close>
+definition maybeM :: "('a \<Rightarrow> ('s, unit) nondet_monad) \<Rightarrow> 'a option \<Rightarrow> ('s, unit) nondet_monad" where
+  "maybeM f y \<equiv> case y of Some x \<Rightarrow> f x | None \<Rightarrow> return ()"
+
 text \<open>Run a sequence of monads from left to right, ignoring return values.\<close>
 definition sequence_x :: "('s, 'a) tmonad list \<Rightarrow> ('s, unit) tmonad" where
   "sequence_x xs \<equiv> foldr (\<lambda>x y. x >>= (\<lambda>_. y)) xs (return ())"
@@ -677,6 +711,48 @@ definition whileLoopE ::
 
 notation (output)
   whileLoopE  ("(whileLoopE (_)//  (_))" [1000, 1000] 1000)
+
+
+section "Combinators that have conditions with side effects"
+
+definition notM :: "('s, bool) nondet_monad \<Rightarrow> ('s, bool) nondet_monad" where
+  "notM m = do c \<leftarrow> m; return (\<not> c) od"
+
+definition
+  whileM :: "('s, bool) nondet_monad \<Rightarrow> ('s, 'a) nondet_monad \<Rightarrow> ('s, unit) nondet_monad" where
+  "whileM C B \<equiv> do
+    c \<leftarrow> C;
+    whileLoop (\<lambda>c s. c) (\<lambda>_. do B; C od) c;
+    return ()
+  od"
+
+definition
+  ifM :: "('s, bool) nondet_monad \<Rightarrow> ('s, 'a) nondet_monad \<Rightarrow> ('s, 'a) nondet_monad \<Rightarrow>
+          ('s, 'a) nondet_monad" where
+  "ifM test t f = do
+    c \<leftarrow> test;
+    if c then t else f
+   od"
+
+definition ifME ::
+  "('a, 'b + bool) nondet_monad \<Rightarrow> ('a, 'b + 'c) nondet_monad \<Rightarrow> ('a, 'b + 'c) nondet_monad
+   \<Rightarrow> ('a, 'b + 'c) nondet_monad" where
+  "ifME test t f = doE
+    c \<leftarrow> test;
+    if c then t else f
+   odE"
+
+definition
+  whenM :: "('s, bool) nondet_monad \<Rightarrow> ('s, unit) nondet_monad \<Rightarrow> ('s, unit) nondet_monad" where
+  "whenM t m = ifM t m (return ())"
+
+definition
+  orM :: "('s, bool) nondet_monad \<Rightarrow> ('s, bool) nondet_monad \<Rightarrow> ('s, bool) nondet_monad" where
+  "orM a b = ifM a (return True) b"
+
+definition
+  andM :: "('s, bool) nondet_monad \<Rightarrow> ('s, bool) nondet_monad \<Rightarrow> ('s, bool) nondet_monad" where
+  "andM a b = ifM a b (return False)"
 
 subsection "Await command"
 
