lib/Monads/trace/Trace_No_Throw.thy
@@ -25,4 +25,74 @@ definition no_throw :: "('s \<Rightarrow> bool) \<Rightarrow> ('s, 'e + 'a) tmon
 definition no_return :: "('a \<Rightarrow> bool) \<Rightarrow> ('a, 'b + 'c) tmonad \<Rightarrow> bool" where
   "no_return P A \<equiv> \<lbrace> P \<rbrace> A \<lbrace>\<lambda>_ _. False\<rbrace>,\<lbrace>\<lambda>_ _. True \<rbrace>"
 
+(* Alternative definition of no_throw; easier to work with than unfolding validE. *)
+lemma no_throw_def':
+  "no_throw P A = (\<forall>s. P s \<longrightarrow> (\<forall>(r, t) \<in> fst (A s). (\<exists>x. r = Inr x)))"
+  by (clarsimp simp: no_throw_def validE_def2 split_def split: sum.splits)
+
+
+lemma no_throw_returnOk[simp]:
+  "no_throw P (returnOk a)"
+  unfolding no_throw_def
+  by wp
+
+lemma no_throw_liftE[simp]:
+  "no_throw P (liftE x)"
+  by (wpsimp simp: liftE_def no_throw_def validE_def)
+
+lemma no_throw_bindE:
+  "\<lbrakk> no_throw A X; \<And>a. no_throw B (Y a); \<lbrace> A \<rbrace> X \<lbrace> \<lambda>_. B \<rbrace>,\<lbrace> \<lambda>_ _. True \<rbrace> \<rbrakk>
+   \<Longrightarrow> no_throw A (X >>=E Y)"
+  unfolding no_throw_def
+  using hoare_validE_cases seqE by blast
+
+lemma no_throw_bindE_simple:
+  "\<lbrakk> no_throw \<top> L; \<And>x. no_throw \<top> (R x) \<rbrakk> \<Longrightarrow> no_throw \<top> (L >>=E R)"
+  using hoareE_TrueI no_throw_bindE by blast
+
+lemma no_throw_handleE_simple:
+  "\<lbrakk> \<And>x. no_throw \<top> L \<or> no_throw \<top> (R x) \<rbrakk> \<Longrightarrow> no_throw \<top> (L <handle> R)"
+  by (fastforce simp: no_throw_def' handleE_def handleE'_def validE_def valid_def bind_def return_def
+                split: sum.splits)
+
+lemma no_throw_handle2:
+  "\<lbrakk> \<And>a. no_throw Y (B a); \<lbrace> X \<rbrace> A \<lbrace> \<lambda>_ _. True \<rbrace>,\<lbrace> \<lambda>_. Y \<rbrace> \<rbrakk> \<Longrightarrow> no_throw X (A <handle2> B)"
+  by (fastforce simp: no_throw_def' handleE'_def validE_def valid_def bind_def return_def
+                split: sum.splits)
+
+lemma no_throw_handle:
+  "\<lbrakk> \<And>a. no_throw Y (B a); \<lbrace> X \<rbrace> A \<lbrace> \<lambda>_ _. True \<rbrace>,\<lbrace> \<lambda>_. Y \<rbrace> \<rbrakk> \<Longrightarrow> no_throw X (A <handle> B)"
+  unfolding handleE_def
+  by (rule no_throw_handle2)
+
+lemma no_throw_fail[simp]:
+  "no_throw P fail"
+  by (clarsimp simp: no_throw_def)
+
+lemma handleE'_nothrow_lhs:
+  "no_throw \<top> L \<Longrightarrow> no_throw \<top> (L <handle2> R)"
+  unfolding no_throw_def
+  using handleE'_wp[rotated] by fastforce
+
+lemma handleE'_nothrow_rhs:
+  "\<lbrakk> \<And>x. no_throw \<top> (R x) \<rbrakk> \<Longrightarrow> no_throw \<top> (L <handle2> R)"
+  unfolding no_throw_def
+  by (metis hoareE_TrueI no_throw_def no_throw_handle2)
+
+lemma handleE_nothrow_lhs:
+  "no_throw \<top> L \<Longrightarrow> no_throw \<top> (L <handle> R)"
+  by (metis handleE'_nothrow_lhs handleE_def)
+
+lemma handleE_nothrow_rhs:
+  "\<lbrakk> \<And>x. no_throw \<top> (R x) \<rbrakk> \<Longrightarrow> no_throw \<top> (L <handle> R)"
+  by (metis no_throw_handleE_simple)
+
+lemma condition_nothrow:
+  "\<lbrakk> no_throw \<top> L; no_throw \<top> R \<rbrakk> \<Longrightarrow> no_throw \<top> (condition C L R)"
+  by (clarsimp simp: condition_def no_throw_def validE_def2)
+
+lemma no_throw_Inr:
+  "\<lbrakk> x \<in> fst (A s); no_throw P A; P s \<rbrakk> \<Longrightarrow> \<exists>y. fst x = Inr y"
+  by (fastforce simp: no_throw_def' split: sum.splits)
+
 end
